Added two simple examples at poST_test

poSTVM/poSTVM_alt_inductive.thy
@@ -145,7 +145,7 @@ inductive
               st\<turnstile>exp2\<rightarrow>val2;
               val = binary_op_exec bin_op val1 val2 \<rbrakk> \<Longrightarrow>
              st\<turnstile>expr.Binary bin_op exp1 exp2\<rightarrow>val"
-  | UnaryOp : "\<lbrakk>st\<turnstile>pexp\<rightarrow>val1;
+  | UnOp : "\<lbrakk>st\<turnstile>pexp\<rightarrow>val1;
                 val = (case un_op of
                         None \<Rightarrow> val1
                       | Some un_op \<Rightarrow> unary_op_exec un_op val1)\<rbrakk> \<Longrightarrow>
@@ -207,95 +207,7 @@ inductive
 
 print_theorems
 
-value "fmempty :: (nat,nat) fmap"
-definition test_process_state1 :: "process_state" where
-"test_process_state1 = 
-  ([stacked_proc_var.Var (fmupd 
-                            ''var1'' 
-                            (stacked_var_init.Symbolic (basic_post_type.Nat 0) None) 
-                          fmempty)],
-  ''state1'',
-  ''state1'',
-  proc_status.Active, 
-  time.Time 0 0 0 0 0)"
 
-definition test_process_state2 :: "process_state" where
-"test_process_state2 = 
-  ([stacked_proc_var.Var (fmupd 
-                            ''var1'' 
-                            (stacked_var_init.Symbolic (basic_post_type.Nat 1) None) 
-                          fmempty)],
-  ''state1'',
-  ''state1'',
-  proc_status.Active, 
-  time.Time 0 0 0 0 0)"
-
-definition test_program_state1 :: "program_state" where
-"test_program_state1 = 
-  ([],
-  (fmupd
-    ''process1''
-    test_process_state1
-    fmempty),
-  ''process1'')"
-
-definition test_program_state2 :: "program_state" where
-"test_program_state2 = 
-  ([],
-  (fmupd
-    ''process1''
-    test_process_state2
-    fmempty),
-  ''process1'')"
-
-definition test_ms1 :: "model_state" where
-"test_ms1 = model_state.ST
-  []
-  ((fmupd
-    ''program1''
-    test_program_state1
-    fmempty),''program1'')
-  []
-  []"
-
-definition test_ms2 :: "model_state" where
-"test_ms2 = model_state.ST
-  []
-  ((fmupd
-    ''program1''
-    test_program_state2
-    fmempty),''program1'')
-  []
-  []"
-
-definition test_statement1 :: "stmt" where
-"test_statement1 = stmt.AssignSt (common_var.Symbolic ''var1'',expr.Const (const.Nat 1))"
-
-
-lemma "(statement_result.Continue,test_ms1)\<turnstile>test_statement1\<longrightarrow>(statement_result.Continue,test_ms2)"
-  apply (simp add: test_statement1_def 
-                test_ms1_def 
-                test_ms2_def 
-                test_process_state1_def
-                test_process_state2_def
-                test_program_state1_def
-                test_program_state2_def)
-  apply (rule AssignS)
-   apply (rule Const)
-   apply (auto)
-  apply (simp add: const_to_basic_def
-set_symbvar_def
-get_cur_var_by_name_def
-set_symbvar_in_ps_in_cur_prog_def
-get_var_by_name.simps
-get_cur_var_list_def
-get_cur_proc_var_list_def
-find_var_by_name_def
-get_cur_var_by_name_def
-get_var_by_name.simps
-get_cur_proc_state_by_prog_def)
-  apply (simp_all)
-  done
 
 (*
 apply (simp add: const_to_basic_def
